ConnectionTable HRR test with Crypto.AE cookies and just one assume (pending fix to LowStar.Buffer.mmalloc)

src/tls/experiments/ConnectionTable/ConnectionTable.fst
@@ -16,6 +16,8 @@ module EE = EverCrypt.Error
 
 open ConnectionTable_Aux
 
+#set-options "--max_fuel 0 --max_ifuel 0 --z3rlimit 30"
+
 // References to connections live in pairwise disjoint regions
 let minv (m:partial_dependent_map maybe_id connection_ref) =
   forall id1 id2.{:pattern (Some? (DM.sel m id1)); (Some? (DM.sel m id2))}
@@ -48,59 +50,57 @@ let connection_inv m c =
   Can't be attached to the table because it needs to dereference connections
 *)
 let inv t h =
-  let m = sel h t in
+  h `contains` t /\
+  (let m = sel h t in
   forall (id:maybe_id).{:pattern (T.defined t id h)}
     (T.defined t id h /\ h `contains` (T.value_of t id h))
-    ==> connection_inv m (sel h (Some?.v (T.sel m id)))
+    ==> connection_inv m (sel h (Some?.v (T.sel m id))))
+
+let framing h0 t l h1 =
+  assert (B.loc_includes (B.loc_all_regions_from true rgn) (B.loc_mreference t));
+  assert (forall (id:maybe_id).{:pattern (T.defined t id h1)}
+    (T.defined t id h1 /\ h1 `contains` (T.value_of t id h1)) ==>
+    B.loc_includes (B.loc_all_regions_from true rgn) 
+                   (B.loc_mreference (T.value_of t id h1)));
+  assert (forall (id:maybe_id).{:pattern (T.defined t id h1)}
+    (T.defined t id h0 /\ h0 `contains` (T.value_of t id h1)) ==>
+    B.loc_includes (B.loc_all_regions_from true rgn) 
+                   (B.loc_mreference (T.value_of t id h0)))
 
 let alloc _ =
-  if model then
-    T.alloc () <: _connection_table
-  else ()
+  if model then T.alloc () <: _connection_table
 
-#set-options "--max_fuel 0 --max_ifuel 0 --z3rlimit 30"
-
-let table : connection_table = 
+let table = 
   recall_region rgn;
   witness_region rgn;
   alloc ()
 
-val key : b:B.lbuffer UInt8.t 16{B.recallable b}
-let key = 
-  B.gcmalloc_of_list
-    cookie_rgn
+// TODO: switch to use the cookie key from TLS.Store,
+// but decrypt is underspecified there.
+let cookie_key =
+  push_frame();
+  let key =
+    B.alloca_of_list
     [ 0x00uy; 0x01uy; 0x02uy; 0x03uy;
       0x04uy; 0x05uy; 0x06uy; 0x07uy;
       0x08uy; 0x09uy; 0x0Auy; 0x0Buy;
-      0x0Cuy; 0x0Duy; 0x0Euy; 0x0Fuy ]
+      0x0Cuy; 0x0Duy; 0x0Euy; 0x0Fuy ] 
+  in
+  let ck =
+    if model then
+      Some (AE.create cookie_rgn alg key phi)
+    else
+      AE.coerce cookie_rgn alg key phi 
+  in
+  pop_frame();
+  ck
 
-let phi s = 
-  Seq.length s >= 32 /\
-  (if model then
-    let random = Seq.slice s 0 32 in
-    let id = id_of_random random in
-    let t:_connection_table = table in
-    token_p t (fun h -> 
-      T.defined t id h /\
-      (let c = T.value_of t id h in
-      token_p c (fun h' -> 
-        Sent_HRR? (sel h' c) /\
-        CH1 random == Sent_HRR?.ch (sel h' c))))
-   else True)
+#push-options "--max_ifuel 1"
 
-let cookie_key : option (k:AE.state alg phi{model ==> AE.safe k}) =
-  B.recall key;
-  if model then
-    Some (AE.create cookie_rgn alg key phi)
-  else
-    AE.coerce cookie_rgn alg key phi
-
-#set-options "--max_fuel 0 --max_ifuel 1 --z3rlimit 10"
-
-let create t id cfg =
+let create id cfg =
   if model then
     begin
-    let t:_connection_table = t in
+    let t:_connection_table = table in
     recall t;
     let h0 = get () in
     let p (id:connection_id{T.defined t id h0}) = frameOf (T.value_of t id h0) in
@@ -110,11 +110,10 @@ let create t id cfg =
   let h0 = get () in
   let rgn1 = new_region rgn in
   let c : mmmref connection rel = ralloc_mm rgn1 (Init cfg) in
-  let h1 = get () in
 
   if model then
     begin
-    let t:_connection_table = t in
+    let t:_connection_table = table in
     assert (forall (id:connection_id).
       T.defined t id h0 ==> ~(c == T.value_of t id h0));
     T.extend t id c;
@@ -123,15 +122,16 @@ let create t id cfg =
       forall (id':connection_id).{:pattern (T.value_of t id' h2)}
         T.defined t id' h2 ==> (T.defined t id' h0 \/ T.value_of t id' h2 == c))
     end;
-    
   c
 
-let free_connection t id c =
+#pop-options
+
+let free_connection id c =
   let h0 = get () in
   rfree c;
   if model then
     let h1 = get () in
-    let t:_connection_table = t in
+    let t:_connection_table = table in
     assert (
       forall (id:connection_id).{:pattern (T.defined t id h1)}
         T.defined t id h1 ==> T.defined t id h0)
@@ -145,7 +145,7 @@ val token_functoriality
 let token_functoriality #a #rel r p q =
   token_functoriality r p q
 
-let receive_client_hello1 t id c ch =
+let receive_client_hello1 id c ch =
   let h0 = get () in
   if ch_compatible ch (Init?.cfg !c) then
     let id0 : maybe_id = if model then 0uy else () in
@@ -154,51 +154,28 @@ let receive_client_hello1 t id c ch =
     c := Sent_HRR ch;
   if model then
     let h1 = get () in
-    let t:_connection_table = t in
+    let t:_connection_table = table in
     assert (
       forall (id:connection_id).{:pattern (T.defined t id h1)}
         T.defined t id h1 ==> T.defined t id h0)
 
-assume val random_of_buffer: b:B.buffer UInt8.t -> ST random
-  (requires  fun h -> B.live h b /\ B.length b >= 32)
-  (ensures   fun h0 r h1 -> h0 == h1 /\ r == Seq.slice (B.as_seq h0 b) 0 32)
+assume
+val _random_of_buffer: b:B.buffer UInt8.t -> ST random
+  (requires fun h -> B.live h b /\ B.length b >= 32)
+  (ensures  fun h0 r h1 -> h0 == h1 /\ r == Seq.slice (B.as_seq h0 b) 0 32)
 
-val validate_cookie':
-    ck:cookie
-  -> Stack (option (maybe_id & random))
-  (requires fun h0 ->
-    Some? cookie_key /\
-    AE.invariant h0 (Some?.v cookie_key) /\ 
-    B.live h0 ck /\
-    (model ==> inv table h0))
-  (ensures  fun h0 o h1 ->
-    B.modifies (AE.footprint (Some?.v cookie_key)) h0 h1 /\
-    AE.invariant h1 (Some?.v cookie_key) /\ 
-    (match o with
-    | None -> True
-    | Some (id, random) ->
-      if model then
-        let t:_connection_table = table in
-        id == id_of_random random /\
-        T.defined t id h0 /\
-        (let c = T.value_of t id h0 in
-           token_p c (fun h ->
-             Sent_HRR? (sel h c) /\
-             CH1 random == Sent_HRR?.ch (sel h c)))
-      else True))
+let random_of_buffer = _random_of_buffer
 
-let validate_cookie' ck =
-  let h0 = get () in
+let validate_cookie ck =
   match cookie_key with
   | None -> None
   | Some cookie_key ->
     begin
+    let h0 = get () in
     push_frame();
     let plain = B.alloca 0uy 64ul in
     let h1 = get () in
     AE.frame_invariant h0 cookie_key B.loc_none h1;
-    assume (B.loc_includes (B.loc_region_only true cookie_rgn) (AE.footprint cookie_key));
-    assume (B.loc_disjoint (AE.footprint cookie_key) (B.loc_buffer ck));
     let res : option (maybe_id & random) =
       match AE.decrypt cookie_key ck 92ul plain with
       | EE.AuthenticationFailure -> None
@@ -206,8 +183,6 @@ let validate_cookie' ck =
         let random = random_of_buffer plain in
         let id = id_of_random random in
         if model then
-          let h2 = get () in
-          assert (phi (B.as_seq h2 plain));
           let t:_connection_table = table in
           recall_p t (fun h -> 
             T.defined t id h /\
@@ -218,43 +193,64 @@ let validate_cookie' ck =
           Some (id, random)
         else Some ((), random)
     in
+    let h3 = get () in
     pop_frame();
-    let h1 = get () in
-    assume (B.modifies B.loc_none h0 h1);
-    AE.frame_invariant h0 cookie_key B.loc_none h1;
+    let h4 = get () in
+    AE.frame_invariant h3 cookie_key (B.loc_region_only false (get_tip h3)) h4;
     res
     end
 
-
-let receive_client_hello2 t id c ch2 =
+let receive_client_hello2 id c ch2 =
   let h0 = get () in
-  match validate_cookie t ch2 with
-  | None -> false
-  | Some id0 -> 
-    if ch_compatible ch2 (Init?.cfg !c) then
+  let CH2 random ck = ch2 in
+  match validate_cookie ck with
+  | None -> 
+    begin
+    let h1 = get() in  
+    assert (
+      if model then
+        let t:_connection_table = table in
+        forall (id:connection_id).{:pattern (T.defined t id h1)}
+          T.defined t id h1 ==> T.defined t id h0
+      else True);
+    false
+    end
+  | Some (id0, random0) -> 
+    let cfg = Init?.cfg !c in
+    if ch_compatible ch2 cfg && random = random0 then
       begin
+      let h0' = get () in
       c := Sent_ServerHello ch2 id0;
       let h1 = get () in
+      AE.frame_invariant h0' (Some?.v cookie_key) (B.loc_mreference c) h1;
       assert (
         if model then
-          let t:_connection_table = t in
+        let t:_connection_table = table in
+        forall (id:connection_id).{:pattern (T.defined t id h1)}
+          T.defined t id h1 ==> T.defined t id h0
+      else True);
+      true
+      end
+    else
+    begin
+      let h1 = get() in  
+      assert (
+        if model then
+          let t:_connection_table = table in
           forall (id:connection_id).{:pattern (T.defined t id h1)}
             T.defined t id h1 ==> T.defined t id h0
         else True);
-      true
+      false
       end
-    else false
 
-
-let receive_client_finished t id c =
+let receive_client_finished id c =
   let c0 = !c in
   let h0 = get() in
-  c := Complete (Sent_ServerHello?.ch c0)
-               (Sent_ServerHello?.id1 c0);
+  c := Complete (Sent_ServerHello?.ch c0) (Sent_ServerHello?.id1 c0);
   let h1 = get () in
   assert (
     if model then
-      let t:_connection_table = t in
+      let t:_connection_table = table in
       forall (id:connection_id).{:pattern (T.defined t id h1)}
         T.defined t id h1 ==> T.defined t id h0
     else True)
