src/tls/experiments/ConnectionTable/ConnectionTable.fsti
@@ -29,10 +29,6 @@ open ConnectionTable_Aux
   We could still store it and keep a witness that the id is the same
   as the index, but this is of little use.
 
-- We could add an API layer that allocates a single global connection table
-  and uses it throughout. We could eliminate that layer by doing this from 
-  the beginning, but avoiding top-level effects is cleaner for an experiment.
-
 - In miTLS, we'll use
 
   type connection_id = random // Unique across clients and server connections
@@ -99,6 +95,16 @@ val empty: m:imap maybe_id connection_ref minv{m == T.empty}
 
 val inv: _connection_table -> mem -> Type0
 
+val framing: h0:mem -> t:_connection_table -> l:B.loc -> h1:mem -> Lemma
+  (requires B.modifies l h0 h1 /\ 
+            B.loc_disjoint l (B.loc_all_regions_from true rgn) /\
+            h0 `contains` t /\
+            (forall a rel (r:mreference a rel). 
+              frameOf r `extends` table_rgn ==> 
+              h1 `contains` r ==> h0 `contains` r) /\
+            inv t h0)
+  (ensures  inv t h1)
+
 inline_for_extraction
 val alloc: unit -> ST connection_table
   (requires fun _ ->
@@ -108,26 +114,48 @@ val alloc: unit -> ST connection_table
     if model then ralloc_post #_ #T.grows rgn empty h0 t h1 /\ inv t h1
     else h0 == h1)
 
+val table : connection_table 
+
+let phi s = 
+  Seq.length s >= 32 /\
+  (if model then
+    let random = Seq.slice s 0 32 in
+    let id = id_of_random random in
+    let t:_connection_table = table in
+    token_p t (fun h -> 
+      T.defined t id h /\
+      (let c = T.value_of t id h in
+      token_p c (fun h' -> 
+        Sent_HRR? (sel h' c) /\
+        CH1 random == Sent_HRR?.ch (sel h' c))))
+   else True)
+
+val cookie_key : k:option (AE.state alg phi){
+  Some? k ==>
+    (let k = Some?.v k in 
+     (model ==> AE.safe k) /\
+     B.loc_includes (B.loc_region_only true cookie_rgn) (AE.footprint k))} 
+
 inline_for_extraction
 val create:
-    t:connection_table
-  -> id:maybe_id
+    id:maybe_id
   -> cfg:configuration
   -> ST (connection_ref id)
   (requires fun h0 ->
     if model then
-      let t:_connection_table = t in
+      let t:_connection_table = table in
       inv t h0 /\ 
       ~(T.defined t id h0)
     else True)
   (ensures  fun h0 c h1 ->
     (if model then 
-      let t:_connection_table = t in
+      let t:_connection_table = table in
       inv t h1 /\
-      mods [Ref t] h0 h1 /\
+      B.modifies (B.loc_mreference t) h0 h1 /\
       T.defined t id h1 /\
       sel h1 t == T.upd (sel h0 t) id c
-     else mods [] h0 h1) /\
+     else 
+       B.modifies B.loc_none h0 h1) /\
     frameOf c `extends` rgn /\
     fresh_region (frameOf c) h0 h1 /\
     ~(h0 `contains` c) /\
@@ -136,21 +164,20 @@ val create:
 
 inline_for_extraction
 val free_connection:
-    t:connection_table
-  -> id:maybe_id
+    id:maybe_id
   -> c:connection_ref id
   -> ST unit
   (requires fun h0 ->
     c `is_live_for_rw_in` h0 /\
     (if model then
-      let t:_connection_table = t in
+      let t:_connection_table = table in
       inv t h0 /\ 
       T.defined t id h0 /\
       T.value_of t id h0 == c
     else True))
   (ensures  fun h0 _ h1 -> 
     (if model then 
-      let t:_connection_table = t in
+      let t:_connection_table = table in
       inv t h1 /\
       T.defined t id h1 /\
       T.value_of t id h0 == c
@@ -159,14 +186,13 @@ val free_connection:
     h1 == HyperStack.free c h0)
 
 val receive_client_hello1:
-    t:connection_table
-  -> id:maybe_id
+    id:maybe_id
   -> c:connection_ref id
   -> ch:client_hello{~(has_cookie ch)}
   -> ST unit
   (requires fun h0 ->
     (if model then
-       let t:_connection_table = t in
+       let t:_connection_table = table in
        inv t h0 /\
        T.defined t id h0 /\
        T.value_of t id h0 == c
@@ -174,9 +200,9 @@ val receive_client_hello1:
     h0 `contains` c /\
     Init? (sel h0 c))
   (ensures  fun h0 _ h1 ->
-    mods [Ref c] h0 h1 /\
+    B.modifies (B.loc_mreference c) h0 h1 /\
     (if model then
-       let t:_connection_table = t in
+       let t:_connection_table = table in
        inv t h1 /\
        T.defined t id h1 /\
        T.value_of t id h1 == c
@@ -186,6 +212,10 @@ val receive_client_hello1:
      else
        sel h1 c == Sent_HRR ch))
 
+val random_of_buffer: b:B.buffer UInt8.t -> ST random
+  (requires fun h -> B.live h b /\ B.length b >= 32)
+  (ensures  fun h0 r h1 -> h0 == h1 /\ r == Seq.slice (B.as_seq h0 b) 0 32)
+
 (*
    Validates a cookie in a second ClientHello.
    In the model, if the cookie is valid we get the connection ID 
@@ -193,41 +223,43 @@ val receive_client_hello1:
    When using appropriate integrity protection, valid cookies must have
    been created and sent in an early HelloRetryRequest.
 *)
-val validate_cookie: t:connection_table -> ch2:client_hello
-  -> Stack (option maybe_id)
+val validate_cookie:
+    ck:cookie
+  -> Stack (option (maybe_id & random))
   (requires fun h0 ->
+    B.frameOf ck == other_rgn /\
     Some? cookie_key /\
     AE.invariant h0 (Some?.v cookie_key) /\ 
-    has_cookie ch2 /\
-    B.live h0 (get_cookie ch2) /\
-    (if model then 
-      let t:_connection_table = t in 
-      inv t h0
-     else True))
+    B.live h0 ck /\
+    (model ==> inv table h0))
   (ensures  fun h0 o h1 ->
     B.modifies (AE.footprint (Some?.v cookie_key)) h0 h1 /\
     AE.invariant h1 (Some?.v cookie_key) /\ 
+    equal_domains h0 h1 /\
     (match o with
     | None -> True
-    | Some id1 ->
+    | Some (id, random) ->
       if model then
-        let t:_connection_table = t in
-        T.defined t id1 h0 /\
-        (let c' = T.value_of t id1 h0 in
-           token_p c' (fun h0 ->
-             Sent_HRR? (sel h0 c') /\
-             ch_of_cookie ch2 == Sent_HRR?.ch (sel h0 c')))
+        let t:_connection_table = table in
+        id == id_of_random random /\
+        T.defined t id h0 /\
+        (let c = T.value_of t id h0 in
+           token_p c (fun h ->
+             Sent_HRR? (sel h c) /\
+             CH1 random == Sent_HRR?.ch (sel h c)))
       else True))
 
 val receive_client_hello2:
-    t:connection_table
-  -> id:maybe_id 
+    id:maybe_id 
   -> c:connection_ref id
-  -> ch2:client_hello
+  -> ch2:client_hello{has_cookie ch2}
   -> ST bool
   (requires fun h0 ->
+    Some? cookie_key /\
+    AE.invariant h0 (Some?.v cookie_key) /\ 
+    B.live h0 (CH2?.ck ch2) /\
     (if model then
-      let t:_connection_table = t in
+      let t:_connection_table = table in
       inv t h0 /\
       T.defined t id h0 /\ 
       T.value_of t id h0 == c
@@ -236,27 +268,29 @@ val receive_client_hello2:
     Init? (sel h0 c) /\ 
     has_cookie ch2)
   (ensures  fun h0 b h1 ->
+    AE.invariant h1 (Some?.v cookie_key) /\ 
     (if model then
-      let t:_connection_table = t in
+      let t:_connection_table = table in
       inv t h1 /\
       T.defined t id h1
     else True) /\
     (let c' = sel h1 c in
-     if b then
-       mods [Ref c] h0 h1 /\
+     if b then      
+       B.modifies (B.loc_union 
+         (AE.footprint (Some?.v cookie_key)) 
+         (B.loc_mreference c)) h0 h1 /\
        Sent_ServerHello? c' /\
        Sent_ServerHello?.ch c' == ch2
      else 
-       mods [] h0 h1))
+       B.modifies (AE.footprint (Some?.v cookie_key)) h0 h1))
 
 val receive_client_finished:
-    t:connection_table
-  -> id:maybe_id
+    id:maybe_id
   -> c:connection_ref id
   -> ST unit
   (requires fun h0 ->
     (if model then
-      let t:_connection_table = t in
+      let t:_connection_table = table in
       inv t h0 /\
       T.defined t id h0 /\ 
       T.value_of t id h0 == c
@@ -264,9 +298,9 @@ val receive_client_finished:
     h0 `contains` c /\
     Sent_ServerHello? (sel h0 c))
   (ensures  fun h0 b h1 ->
-    mods [Ref c] h0 h1 /\
+    B.modifies (B.loc_mreference c) h0 h1 /\
     (if model then
-      let t:_connection_table = t in
+      let t:_connection_table = table in
       inv t h1 /\
       T.defined t id h1
     else True) /\
