src/tls/experiments/ConnectionTable/ConnectionTable_Aux.fst
@@ -14,6 +14,7 @@ let cookie = c:AE.cipher_p alg
 
 let cookie_rgn = Mem.tls_define_region
 let table_rgn  = Mem.tls_tables_region
+let other_rgn  = Mem.tls_psk_region
 
 let random = Seq.lseq UInt8.t 32
 
@@ -23,7 +24,7 @@ let id_of_random (r:random) : connection_id =
 noeq
 type client_hello =
   | CH1: random -> client_hello
-  | CH2: random -> ck:cookie{B.frameOf ck == cookie_rgn} -> client_hello
+  | CH2: random -> ck:cookie{B.frameOf ck == other_rgn} -> client_hello
 
 let ch_random = function
   | CH1 r -> r
@@ -39,7 +40,7 @@ let ch_of_cookie (ch:client_hello{has_cookie ch}) =
   let CH2 random _ = ch in
   CH1 random
 
-let ch_compatible ch cfg = true
+val ch_compatible: ch:client_hello -> cfg:configuration -> bool
+let ch_compatible ch cfg = false
 
 let rgn = table_rgn
-
