src/tls/experiments/ConnectionTable/Test.fst
@@ -5,43 +5,109 @@ open ConnectionTable
 
 open FStar.HyperStack.ST
 
+module T = FStar.Monotonic.DependentMap
+module B = LowStar.Buffer
+module AE = Crypto.AEAD
+module HS = FStar.HyperStack
+
 #set-options "--z3rlimit 100 --max_fuel 0 --max_ifuel 0"
+
+(* Added a pattern; all alternatives I tried didn't work or were too cumbersome *)
+val token_functoriality
+  (#a:Type0) (#rel:Preorder.preorder a) (r:mreference a rel)
+  (p:mem_predicate{token_p r p}) (q:mem_predicate{forall (h:HS.mem). p h ==> q h})
+  : Lemma (token_p r q)
+   [SMTPat (token_p r p); SMTPat (token_p r q)]
+let token_functoriality #a #rel r p q =
+  token_functoriality r p q
+
+val frame_invariant
+  (h: HS.mem) (s: AE.state alg phi)
+  (l: B.loc) (h' : HS.mem)
+: Lemma
+  (requires B.modifies l h h' /\ B.loc_disjoint l (AE.footprint s) /\ AE.invariant h s)
+  (ensures  AE.invariant h' s)
+  [SMTPat (AE.invariant h s); SMTPat (B.modifies l h h')] 
+let frame_invariant h s l h' =
+  AE.frame_invariant h s l h'
 
 (*
    This tests the server side of a full handshake with mismatched parameters:
 
-   1. Allocate an empty connection table
+   1. Assume the global connection table is empty
    2. Create a first connection c1 with id = 1 (in Init state)
-   3. Receive a ClientHello ch1 on c1. Transition c1 to Sent_HRR 0 ch1
+   3. Receive a ClientHello ch1 on c1. Transition c1 to Sent_HRR ch1
    4. Deallocate c1
    5. Create a second connection c2 with the same configuration (in Init state)
-   6. Receive a ClientHello ch2 on c2 with a cookie extension matching ch1.
+   6. Create a cookie matching ch1 and encrypt it using Crypto.AE
+   7. Receive a ClientHello ch2 with this cookie on c2.
    7. If the configuration of c2 is compatible with ch2,
       a. Transition c2 to Sent_ServerHello ch2 1, with c1 as the matching 
          initial connection
       b. Receive a ClientFinished on c2 and transition c2 to Complete ch2 1
    8. Deallocate c2
+   
+   The connection table invariant is preserved throughout. 
+   For example, before deallocating c2 we can prove there was a matching
+   connection in the table that ended in Sent_HRR state, even if it was freed.
 *)
-module T = FStar.Monotonic.DependentMap
 
-let test
-  (cfg:configuration)
-  (ch1:client_hello{~(has_cookie ch1)})
-  (ch2:client_hello{has_cookie ch2})
-: ST connection_table
-  (requires fun _ ->
-    witnessed (region_contains_pred rgn) /\ ch_of_cookie ch2 == ch1 /\
-    ~(ch_compatible ch1 cfg))
-  (ensures  fun _ t h1 -> model ==> inv t h1)
-=
-  let id1 = if model then 1ul else () in
-  let id2 = if model then 2ul else () in
-  let t = alloc () in
-  let c1 = create t id1 cfg in
-  receive_client_hello1 t id1 c1 ch1;
-  free_connection t id1 c1;
+val test (cfg:configuration) : ST unit 
+  (requires fun h0 ->
+    Some? cookie_key /\
+    AE.invariant h0 (Some?.v cookie_key) /\ 
+    (if model then
+      let t : _connection_table = table in
+      inv t h0 /\
+      HS.contains h0 t /\ 
+      HS.sel h0 t == T.empty
+    else True) /\
+    witnessed (region_contains_pred rgn))
+  (ensures  fun _ t h1 -> model ==> inv table h1)
+
+let test cfg =
+  let h0 = get () in
+  let id1 = if model then 1uy else () in
+  let id2 = if model then 2uy else () in
+  let c1 = create id1 cfg in
+  let ch1 = CH1 (Seq.create 32 1uy) in
+  receive_client_hello1 id1 c1 ch1;  
+  if model then
+    begin
+    let s = Seq.create 64 1uy in
+    let random = Seq.slice s 0 32 in
+    let id = id_of_random random in  
+    let t : _connection_table = table in
+    assert (Seq.eq random (Seq.create 32 1uy));
+    T.contains_stable t 1uy c1;
+    witness_p c1 (fun h' -> 
+      Sent_HRR? (HS.sel h' c1) /\
+      CH1 random == Sent_HRR?.ch (HS.sel h' c1));
+    witness_p t (fun h -> 
+      T.contains t id c1 h /\
+      token_p c1 (fun h' ->
+        Sent_HRR? (HS.sel h' c1) /\
+        CH1 random == Sent_HRR?.ch (HS.sel h' c1)));
+    assert (phi s)
+    end;
+  free_connection id1 c1;
+  let c2 = create id2 cfg in
   let h1 = get () in
-  let c2 = create t id2 cfg in
-  if receive_client_hello2 t id2 c2 ch2 then receive_client_finished t id2 c2;
-  free_connection t id2 c2;
-  t
+  let plain = B.malloc other_rgn 1uy 64ul in
+  let ck = B.malloc other_rgn 0uy 92ul in
+  let h2 = get () in  
+  //AE.frame_invariant h0 (Some?.v cookie_key) (B.loc_all_regions_from true rgn) h2;
+  Crypto.AE.encrypt (Some?.v cookie_key) plain 64ul ck;
+  let ch2 = CH2 (Seq.create 32 0uy) ck in
+  let h3 = get () in
+  if model then
+    begin
+    let t : _connection_table = table in
+    // malloc seems underspecified. It can allocate other buffers in other regions
+    assume (forall a rel (r:mreference a rel). 
+      HS.frameOf r `HS.extends` table_rgn ==> 
+      h2 `HS.contains` r ==> h1 `HS.contains` r);
+    framing h1 t (B.loc_union (AE.footprint (Some?.v cookie_key)) (B.loc_buffer ck)) h3
+    end;
+  if receive_client_hello2 id2 c2 ch2 then receive_client_finished id2 c2;
+  free_connection id2 c2
